Adapted destuttering proof to work with ext transitions

fairness/ext_models/destutter_ext.v
@@ -6,6 +6,18 @@ From trillium.fairness Require Export fuel lm_fair.
 From trillium.fairness.ext_models Require Export ext_models.
 (* ext_lm_fair.  *)
 
+
+(* TODO: move to lm_fair, reorganize?, reduce the scope? *)
+Class LMFairPre `{LM: LiveModel G M LSI} := {
+  edG :> EqDecision G;
+  cntG :> Countable G;
+  edM :> EqDecision (fmstate M);
+  dTr :> ∀ s1 ρ s2, Decision (fmtrans M s1 (Some ρ) s2);
+  inhLM :> Inhabited (lm_ls LM);
+  inhG :> Inhabited G;
+}. 
+
+
 Section ExtLM.
   (** The differences with Ext(LM_Fair) are:
       - this is not a FairModel, so there is no notion of "roles" and enabledness
@@ -14,32 +26,70 @@ Section ExtLM.
       would be hard to conduct using LM_Fair-like traces *)
 
   Context `{LM: LiveModel G M LSI}.
-  Context `{EM: ExtModel M}.
+  Context {LMFP: LMFairPre (LM := LM)}.
+  Let LMF := LM_Fair (LM := LM).
+  
+  Context {ELMF: ExtModel LMF}.
 
-  Context `{Countable G} `{EqDecision M}.
-  Context `{∀ s1 ρ s2, Decision (fmtrans M s1 (Some ρ) s2)}.
-  Context `{Inhabited (lm_ls LM)} `{Inhabited G}.
-  Let LMF := LM_Fair (LM := LM). 
-  Context `{ELMF: ExtModel LMF}.
-
-  Definition elm_role := (lm_lbl LM + (@EI _ ELMF))%type. 
+  Definition elm_lbl := (lm_lbl LM + (@EI _ ELMF))%type. 
 
   (* TODO: change name? *)
-  Inductive elm_trans: lm_ls LM -> elm_role -> lm_ls LM -> Prop :=
+  Inductive elm_trans: lm_ls LM -> elm_lbl -> lm_ls LM -> Prop :=
   | elm_lm_step s1 ℓ s2 (STEP: lm_ls_trans LM s1 ℓ s2):
     elm_trans s1 (inl ℓ) s2
   | elm_ext_step s1 s2 ι (REL: ETs ι s1 s2):
     elm_trans s1 (inr ι) s2.   
 
+  Definition ELM : Model := {|
+    mstate := lm_ls LM;
+    mlabel := elm_lbl;
+    mtrans := elm_trans
+  |}.  
+
+  Definition eauxtrace := trace (mstate ELM) (mlabel ELM). 
+
+  CoInductive eauxtrace_valid: eauxtrace -> Prop :=
+  | eauxtrace_valid_singleton δ: eauxtrace_valid ⟨δ⟩
+  | eauxtrace_valid_cons δ ℓ tr:
+      elm_trans δ ℓ (trfirst tr) ->
+      eauxtrace_valid tr →
+      eauxtrace_valid (δ -[ℓ]-> tr).
+
+  (* TODO: unify fairness definitions by parametrizing fair_by
+     with predicate on "expected step"; use it in fair_aux and fair_eaux  *)
+  Definition fair_eaux ρ (eauxtr: eauxtrace): Prop :=
+    forall n, pred_at eauxtr n (λ δ _, role_enabled ρ δ) ->
+         ∃ m, pred_at eauxtr (n+m) (λ δ _, ¬role_enabled ρ δ) ∨
+              pred_at eauxtr (n+m) (λ _ ℓ, ∃ tid, ℓ = Some $ inl (Take_step ρ tid)).
+
+  (* TODO: remove after refactoring of fair_eaux*)
+  Lemma fair_eaux_after ρ eauxtr n eauxtr':
+    fair_eaux ρ eauxtr ->
+    after n eauxtr = Some eauxtr' ->
+    fair_eaux ρ eauxtr'.
+  Proof.
+    rewrite /fair_aux => Hfair Hafter m Hpa.
+    specialize (Hfair (n+m)).
+    rewrite -> (pred_at_sum _ n) in Hfair. rewrite Hafter in Hfair.
+    destruct (Hfair Hpa) as (p&Hp).
+    exists (p). by rewrite <-Nat.add_assoc, ->!(pred_at_sum _ n), Hafter in Hp.
+  Qed.
+
 End ExtLM.
 
 
-Section fuel_dec_unless.
-  Context `{LM: LiveModel G Mdl LSI}.
-  Context `{Countable G}.
+Section destuttering_auxtr.
+  Context `{LM: LiveModel G M LSI}.
+  Context {EM: ExtModel M}.
+  (* Let EMF := ext_model_FM (EM := EM).  *)
+  Context {LMFP: LMFairPre (LM := LM)}.
+  Let LMF := LM_Fair (LM := LM).
+  Context {ELMF: ExtModel LMF}.
+
+  Context (proj_ext: (@EI _ ELMF) -> (@EI _ EM)). 
   
   Lemma fuel_must_not_incr_fuels oρ'
-    (δ1 δ2: LiveState G Mdl LSI)
+    (δ1 δ2: LiveState G M LSI)
     ρ f1 f2
     (KEEP: fuel_must_not_incr oρ' δ1 δ2)
     (FUEL1: ls_fuel δ1 !! ρ = Some f1)
@@ -55,7 +105,7 @@ Section fuel_dec_unless.
   Qed.
 
   Lemma step_nonincr_fuels ℓ
-    (δ1 δ2: LiveState G Mdl LSI)
+    (δ1 δ2: LiveState G M LSI)
     ρ f1 f2
     (STEP: lm_ls_trans LM δ1 ℓ δ2)
     (FUEL1: ls_fuel δ1 !! ρ = Some f1)
@@ -68,27 +118,28 @@ Section fuel_dec_unless.
   Qed. 
 
 
-  Definition Ul (ℓ: LM.(mlabel)) :=
+  Definition EUl (ℓ: ELM.(mlabel)): option (option (@ext_role _ EM)) :=
     match ℓ with
-    | Take_step ρ _ => Some (Some ρ)
+    | inl (Take_step ρ _) => Some (Some (inl ρ))
+    | inr e => Some $ Some $ inr $ env $ proj_ext $ e
     | _ => None
     end.
 
-  Definition Ψ (δ: LiveState G Mdl LSI) :=
+  Definition Ψ (δ: LiveState G M LSI) :=
     size δ.(ls_fuel) + [^ Nat.add map] ρ ↦ f ∈ δ.(ls_fuel (G := G)), f.
 
-  Lemma fuel_dec_unless0 δ ℓ (auxtr' : trace (lm_ls LM) (lm_lbl LM))
-    (Hval : auxtrace_valid (δ -[ ℓ ]-> auxtr')):
-  (∃ ℓ' : option (fmrole Mdl), Ul ℓ = Some ℓ')
-  ∨ Ψ (trfirst auxtr') < Ψ δ ∧ ls_under δ = ls_under $ trfirst auxtr'.
-  Proof.
-    inversion Hval as [|??? Htrans Hmatch]; simplify_eq =>//.
+  Lemma fuel_dec_unless_lm_step δ ℓ δ'
+    (Htrans : lm_ls_trans LM δ ℓ δ'):
+    (∃ ℓ' : fmrole M, EUl (inl ℓ) = Some $ Some $ inl ℓ') ∨
+    Ψ δ' < Ψ δ ∧ ls_under δ = ls_under δ'.
+  Proof. 
     destruct ℓ as [| tid' |];
       [left; eexists; done| right | inversion Htrans; naive_solver ].
+
     destruct Htrans as (Hne&Hdec&Hni&Hincl&Heq).
     rewrite -> Heq in *. split; last done.
-
-    destruct (decide (dom $ ls_fuel δ = dom $ ls_fuel (trfirst auxtr'))) as [Hdomeq|Hdomneq].
+    
+    destruct (decide (dom $ ls_fuel δ = dom $ ls_fuel δ')) as [Hdomeq|Hdomneq].
     - destruct Hne as [ρ Hρtid].
 
       assert (ρ ∈ dom $ ls_fuel δ) as Hin by rewrite -ls_same_doms elem_of_dom //.
@@ -98,55 +149,61 @@ Section fuel_dec_unless.
       rewrite /Ψ -!size_dom Hdomeq.
       apply Nat.add_lt_mono_l.
 
-      rewrite /Ψ (big_opM_delete (λ _ f, f) (ls_fuel (trfirst _)) ρ) //.
+      rewrite /Ψ (big_opM_delete (λ _ f, f) (ls_fuel δ') ρ) //.
       rewrite (big_opM_delete (λ _ f, f) (ls_fuel  δ) ρ) //.
       apply Nat.add_lt_le_mono.
       { rewrite /fuel_decr in Hdec. specialize (Hdec ρ). rewrite Hf Hf' /= in Hdec.
         apply Hdec; [set_solver | set_solver | by econstructor]. }
-
       apply big_addM_leq_forall => ρ' Hρ'.
       rewrite dom_delete_L in Hρ'.
       have Hρneqρ' : ρ ≠ ρ' by set_solver.
       rewrite !lookup_delete_ne //.
       destruct (decide (ρ' ∈ dom δ.(ls_fuel))) as [Hin|Hnotin]; last set_solver.
       rewrite /fuel_must_not_incr in Hni.
-      (* destruct (Hni ρ' ltac:(done) ltac:(done)); [done|set_solver]. *)
       destruct (Hni ρ' ltac:(done)); [done|set_solver].
-    - assert (size $ ls_fuel (trfirst auxtr') < size $ ls_fuel δ).
+    - assert (size $ ls_fuel δ' < size $ ls_fuel δ).
       { rewrite -!size_dom. apply subset_size. set_solver. }
       apply Nat.add_lt_le_mono =>//.
       apply big_addM_leq_forall => ρ' Hρ'.
-      (* destruct (Hni ρ' ltac:(set_solver) ltac:(done)); [done|set_solver]. *)
       destruct (Hni ρ' ltac:(set_solver)); [done|set_solver].
-  Qed. 
-
-  Lemma fuel_dec_unless (auxtr: auxtrace (LM := LM)) :
-    auxtrace_valid auxtr ->
-    dec_unless ls_under Ul Ψ auxtr.
-  Proof.
-    intros Hval n. revert auxtr Hval. induction n; intros auxtr Hval; last first.
-    { edestruct (after (S n) auxtr) as [auxtrn|] eqn:Heq; rewrite Heq =>//.
-      simpl in Heq. simplify_eq. destruct auxtrn as [|δ ℓ auxtr']=>//; last first.
-      inversion Hval as [|???? Hmatch]; simplify_eq =>//.
-      specialize (IHn _ Hmatch). rewrite Heq // in IHn. }
-    rewrite after_0_id. destruct auxtr; [done| ].
-    by apply fuel_dec_unless0. 
   Qed.
 
-End fuel_dec_unless.
+  Lemma fuel_dec_unless_step δ ℓ δ'
+    (Htrans : elm_trans δ ℓ δ'):
+    (∃ ℓ' : option (@ext_role _ EM), EUl ℓ = Some ℓ') ∨
+    Ψ δ' < Ψ δ ∧ ls_under δ = ls_under δ'.
+  Proof. 
+    inversion Htrans.
+    { subst. eapply fuel_dec_unless_lm_step in STEP; eauto.
+      destruct STEP as [[? STEP]| ?]; [| tauto].
+      left. eauto. }
+    subst.
+    left. eauto.
+  Qed.
 
-Section destuttering_auxtr.
-  Context `{LM: LiveModel G M LSI}.
+  Lemma fuel_dec_unless
+    (* (auxtr: auxtrace (LM := LM)) *)
+          (eauxtr: eauxtrace (LM := LM))
+    :
+    eauxtrace_valid eauxtr ->
+    dec_unless ls_under EUl Ψ eauxtr.
+  Proof.
+    intros Hval n. revert eauxtr Hval. induction n; intros eauxtr Hval; last first.
+    { edestruct (after (S n) eauxtr) as [eauxtrn|] eqn:Heq; rewrite Heq =>//.
+      simpl in Heq. simplify_eq. destruct eauxtrn as [|δ ℓ eauxtr']=>//; last first.
+      inversion Hval as [|???? Hmatch]; simplify_eq =>//.
+      specialize (IHn _ Hmatch). rewrite Heq // in IHn. }
+    rewrite after_0_id. destruct eauxtr; [done| ].
+    inversion Hval as [|??? Htrans Hmatch]; simplify_eq =>//.
+    eapply fuel_dec_unless_step; eauto. 
+  Qed.
 
-  Context `{Countable G}.
+  Definition upto_stutter_eauxtr :=
+    upto_stutter (ls_under (G:=G) (M:=M) (LSI := LSI)) EUl.
 
-  (* Why is [LM] needed here? *)
-  Definition upto_stutter_auxtr :=
-    upto_stutter (ls_under (G:=G) (M:=M) (LSI := LSI)) (Ul (LM := LM)).
-
-  Lemma can_destutter_auxtr auxtr:
-    auxtrace_valid auxtr →
-    ∃ mtr, upto_stutter_auxtr auxtr mtr.
+  Lemma can_destutter_eauxtr eauxtr:
+    eauxtrace_valid eauxtr →
+    ∃ mtr, upto_stutter_eauxtr eauxtr mtr.
   Proof.
     intros ?. eapply can_destutter.
     eapply fuel_dec_unless =>//.
@@ -154,34 +211,61 @@ Section destuttering_auxtr.
 
 End destuttering_auxtr.
 
+(* TODO: move *)
+Lemma upto_stutter_mono' {S S' L L': Type} (Us: S -> S') (Ul: L -> option L'):
+  monotone2 (upto_stutter_ind Us Ul).
+Proof.
+  unfold monotone2. intros x0 x1 r r' IN LE.
+  induction IN; try (econstructor; eauto; done).
+Qed.
+
 Section upto_preserves.
+  (* Context `{LM: LiveModel G M LSI}. *)
+  (* Context `{Countable G}. *)
   Context `{LM: LiveModel G M LSI}.
-  Context `{Countable G}.
+  Context {EM: ExtModel M}.
+  Context {LMFP: LMFairPre (LM := LM)}.
+  Let LMF := LM_Fair (LM := LM).
+  Context {ELMF: ExtModel LMF}.
+  Context (proj_ext: (@EI _ ELMF) -> (@EI _ EM)). 
 
-  Lemma upto_stutter_mono' :
-    monotone2 (upto_stutter_ind (ls_under (LSI := LSI)) (Ul (LM:=LM))).
-  Proof.
-    unfold monotone2. intros x0 x1 r r' IN LE.
-    induction IN; try (econstructor; eauto; done).
-  Qed.
-  Hint Resolve upto_stutter_mono' : paco.
+  Hypothesis PROJ_KEEP_EXT:
+    forall δ1 ι δ2, (@ETs _ ELMF) ι δ1 δ2 -> 
+                (@ETs _ EM) (proj_ext ι) (ls_under δ1) (ls_under δ2). 
 
-  Lemma upto_preserves_validity (auxtr : auxtrace (LM := LM)) mtr:
-    upto_stutter_auxtr auxtr mtr ->
-    auxtrace_valid auxtr ->
-    mtrace_valid mtr.
+  Local Hint Resolve upto_stutter_mono' : paco.
+
+  (* TODO: here and for similar lemmas:
+     try to unify usual and external versions *)
+  Lemma upto_preserves_validity (eauxtr : eauxtrace (LM := LM)) mtr:
+    upto_stutter_eauxtr proj_ext eauxtr mtr ->
+    eauxtrace_valid eauxtr ->
+    emtrace_valid mtr.
   Proof.
-    revert auxtr mtr. pcofix CH. intros auxtr mtr Hupto Hval.
+    revert eauxtr mtr. pcofix CH. intros eauxtr mtr Hupto Hval.
     punfold Hupto.
     induction Hupto as [| |btr str δ ????? IH].
     - pfold. constructor.
     - apply IHHupto. inversion Hval. assumption.
     - pfold; constructor=>//.
-      + subst. inversion Hval as [| A B C Htrans E F ] =>//. subst. unfold ls_trans in *.
-        destruct ℓ; try done. simpl in *. simplify_eq.
-        destruct Htrans as [??].
-        have <- //: ls_under $ trfirst btr = trfirst str.
-        { destruct IH as [IH|]; last done. punfold IH. inversion IH =>//. }
+      + subst. inversion Hval as [| A B C Htrans E F ] =>//. subst.
+
+        inversion Htrans.
+        * subst.  
+          unfold lm_ls_trans, ls_trans in *.
+          destruct ℓ0; try done. simpl in *. simplify_eq.
+          destruct STEP as [??].
+          have <- //: ls_under $ trfirst btr = trfirst str.
+          { destruct IH as [IH|]; last done. punfold IH. inversion IH =>//. }
+          by constructor. 
+        * subst.
+          simpl in H0. inversion H0. subst. 
+          constructor.
+          replace (trfirst str) with (ls_under (trfirst btr)).
+          2: { (* TODO: a faster way? *)
+               inversion IH; [| pclearbot; done].
+               symmetry. eapply upto_stutter_trfirst; eauto. }           
+          eapply PROJ_KEEP_EXT; eauto. 
       + right. eapply CH.
         { destruct IH =>//. }
         subst. by inversion Hval.
@@ -190,110 +274,71 @@ Section upto_preserves.
 End upto_preserves.
 
 Section upto_stutter_preserves_fairness_and_termination.
+  (* Context `{LM: LiveModel G M LSI}. *)
+  (* Context `{Countable G}. *)
   Context `{LM: LiveModel G M LSI}.
-  Context `{Countable G}.
+  Context {EM: ExtModel M}.
+  Context {LMFP: LMFairPre (LM := LM)}.
+  Let LMF := LM_Fair (LM := LM).
+  Context {ELMF: ExtModel LMF}.
+  Context (proj_ext: (@EI _ ELMF) -> (@EI _ EM)). 
 
-  Notation upto_stutter_aux := (upto_stutter (ls_under (LSI := LSI)) (Ul (LM := LM))).
+  (* Notation upto_stutter_aux := (upto_stutter (ls_under (LSI := LSI)) (Ul (LM := LM))). *)
 
-  Lemma upto_stutter_mono'' : (* TODO fix this proliferation *)
-    monotone2 (upto_stutter_ind (ls_under (LSI := LSI)) (Ul (LM:=LM))).
-  Proof.
-    unfold monotone2. intros x0 x1 r r' IN LE.
-    induction IN; try (econstructor; eauto; done).
-  Qed.
-  Hint Resolve upto_stutter_mono' : paco.
-
-  Lemma upto_stutter_step_correspondence auxtr (mtr: mtrace M)
-    (Po: LiveState _ _ LSI -> option (mlabel LM) -> Prop)
-    (Pi: M -> option (option (fmrole M)) -> Prop)
+  Lemma upto_stutter_step_correspondence (eauxtr: eauxtrace (LM := LM)) (emtr: emtrace (EM := EM))
+    (Po: LiveState _ _ LSI -> option (mlabel ELM) -> Prop)
+    (Pi: M -> option (option (ext_role (EM := EM))) -> Prop)
     (LIFT: forall δ oℓ, Po δ oℓ -> Pi (ls_under δ) (match oℓ with 
-                                              | Some ℓ => Ul ℓ (LM := LM)
+                                              | Some ℓ => EUl proj_ext ℓ (LM := LM)
                                               | None => None
                                               end))
     (PI0: forall st, Pi st None -> forall ℓ, Pi st (Some ℓ))
     :
-    upto_stutter_auxtr auxtr mtr (LM := LM) ->
+    upto_stutter_eauxtr proj_ext eauxtr emtr (LM := LM) ->
     forall n atr_aux,
-      after n auxtr = Some atr_aux ->
+      after n eauxtr = Some atr_aux ->
       pred_at atr_aux 0 Po ->
     exists m atr_m,
-      after m mtr = Some atr_m /\ pred_at atr_m 0 Pi /\ 
-      upto_stutter_auxtr atr_aux atr_m.
+      after m emtr = Some atr_m /\ pred_at atr_m 0 Pi /\ 
+      upto_stutter_eauxtr proj_ext atr_aux atr_m.
   Proof.
-    intros Hupto n. generalize dependent auxtr. generalize dependent mtr. 
-    induction n as [|n]; intros auxtr mtr Hupto atr_aux AFTER A0.
-    - rewrite after_0_id in AFTER. assert (atr_aux = mtr) as -> by congruence.
+    intros Hupto n. generalize dependent eauxtr. generalize dependent emtr. 
+    induction n as [|n]; intros eauxtr emtr Hupto atr_aux AFTER A0.
+    - rewrite after_0_id in AFTER. assert (atr_aux = emtr) as -> by congruence.
       do 2 eexists. split; [| split]; [..| by eauto].
       { by erewrite after_0_id. }
       punfold Hupto. inversion Hupto; simplify_eq.
+      4: { apply upto_stutter_mono'. }
       + rename A0 into Hpa.
         rewrite /pred_at /=. rewrite /pred_at //= in Hpa.
         by apply LIFT in Hpa. 
       + rewrite -> !pred_at_0 in A0.
-        rewrite /pred_at /=. destruct auxtr; simpl in *; try congruence.
+        rewrite /pred_at /=. destruct eauxtr; simpl in *; try congruence.
         * apply LIFT in A0. congruence.
         * apply LIFT in A0. destruct ℓ; simpl in *; try done.
+          destruct l; [done| ..].           
           all: subst; eapply PI0; eauto.
       + rewrite -> !pred_at_0 in A0.
-        apply pred_at_0. rewrite <- H1.
+        apply pred_at_0. rewrite <- H0.
         by eapply LIFT in A0. 
     - punfold Hupto. inversion Hupto as [| |?????? ?? IH ]; simplify_eq.
+      3: { apply upto_stutter_mono'. }
       + simpl in AFTER. 
         eapply IHn; eauto.
         by pfold.
       + simpl in AFTER.
-        assert (upto_stutter_auxtr btr str) as UPTO'.
+        assert (upto_stutter_eauxtr proj_ext btr str) as UPTO'.
         { inversion IH; eauto. done. } 
         specialize (IHn str btr UPTO' _ AFTER A0) as (m & ?&?&?).
         exists (S m). eauto. 
   Qed.
 
-  (* Lemma upto_stutter_fairness_0 ρ auxtr (mtr: mtrace M): *)
-  (*   upto_stutter_aux auxtr mtr -> *)
-  (*   (* role_enabled_model ρ (trfirst mtr) -> *) *)
-  (*   (∃ n, pred_at auxtr n (λ δ _, ¬role_enabled (G := G) ρ δ) *)
-  (*         ∨ pred_at auxtr n (λ _ ℓ, ∃ ζ, ℓ = Some (Take_step ρ ζ))) -> *)
-  (*   ∃ m, pred_at mtr m (λ δ _, ¬role_enabled_model ρ δ) *)
-  (*        ∨ pred_at mtr m (λ _ ℓ, ℓ = Some $ Some ρ). *)
-  (*   Proof. *)
-  (*     intros Hupto (* Hre *) [n Hstep]. *)
-  (*     revert auxtr mtr Hupto (* Hre *) Hstep. *)
-  (*     induction n as [|n]; intros auxtr mtr Hupto (* Hre *) Hstep. *)
-  (*     - punfold Hupto. inversion Hupto; simplify_eq. *)
-  (*       + destruct Hstep as [Hpa|[??]]; try done. *)
-  (*         exists 0. left. rewrite /pred_at /=. rewrite /pred_at //= in Hpa. *)
-  (*       + rewrite -> !pred_at_0 in Hstep. exists 0. *)
-  (*         destruct Hstep as [Hstep| [tid Hstep]]; [left|right]. *)
-  (*         * rewrite /pred_at /=. destruct mtr; simpl in *; try congruence. *)
-  (*         * exfalso. injection Hstep => Heq. rewrite -> Heq in *. *)
-  (*           unfold Ul in *. congruence. *)
-  (*       + rewrite -> !pred_at_0 in Hstep. exists 0. *)
-  (*         destruct Hstep as [Hstep| [tid Hstep]]; [left|right]. *)
-  (*         * rewrite /pred_at //=. *)
-  (*         * rewrite /pred_at //=. injection Hstep. intros Heq. simplify_eq. *)
-  (*           unfold Ul in *. congruence. *)
-  (*     - punfold Hupto. inversion Hupto as [| |?????? ?? IH ]; simplify_eq. *)
-  (*       + destruct Hstep as [?|?]; done. *)
-  (*       + rewrite -> !pred_at_S in Hstep. *)
-  (*         eapply IHn; eauto. *)
-  (*         by pfold. *)
-  (*       + destruct (decide (ℓ' = Some ρ)). *)
-  (*         * simplify_eq. *)
-  (*           exists 0. right. rewrite pred_at_0 //. *)
-  (*         * have Hw: ∀ (P: nat -> Prop), (∃ n, P (S n)) -> (∃ n, P n). *)
-  (*           { intros P [x ?]. by exists (S x). } *)
-  (*           apply Hw. setoid_rewrite pred_at_S. *)
-  (*           eapply IHn; eauto. *)
-  (*           { destruct IH as [|]; done. } *)
-  (*   Qed. *)
-
-
-  Lemma upto_stutter_fairness_0 ρ auxtr (mtr: mtrace M):
-    upto_stutter_aux auxtr mtr ->
-    (∃ n, pred_at auxtr n (λ δ _, ¬role_enabled (LSI := LSI) ρ δ)
-          ∨ pred_at auxtr n (λ _ ℓ, ∃ ζ, ℓ = Some (Take_step ρ ζ))) ->
+  Lemma upto_stutter_fairness_0 ρ eauxtr (mtr: emtrace (EM := EM)):
+    upto_stutter_eauxtr proj_ext eauxtr mtr ->
+    (∃ n, pred_at eauxtr n (λ δ _, ¬role_enabled (LSI := LSI) ρ δ)
+          ∨ pred_at eauxtr n (λ _ ℓ, ∃ ζ, ℓ = Some $ inl (Take_step ρ ζ))) ->
     ∃ m, pred_at mtr m (λ δ _, ¬role_enabled_model ρ δ)
-         ∨ pred_at mtr m (λ _ ℓ, ℓ = Some $ Some ρ).
+         ∨ pred_at mtr m (λ _ ℓ, ℓ = Some $ Some $ inl ρ).
   Proof.
     repeat setoid_rewrite <- pred_at_or. 
     intros UPTO [n NTH].
@@ -304,36 +349,66 @@ Section upto_stutter_preserves_fairness_and_termination.
     - destruct NTH as (m & atr_m & AFTERm & Pm & UPTO').
       exists m. rewrite (plus_n_O m) pred_at_sum AFTERm. apply Pm. 
     - intros ?? Po. destruct Po as [?| [? ->]]; eauto.
-    - intros. destruct H0; [| done]. eauto.
-  Qed.  
-    
-  Lemma upto_stutter_fairness (auxtr:auxtrace (LM := LM)) (mtr: mtrace M):
-    upto_stutter_aux auxtr mtr ->
-    (∀ ρ, fair_aux ρ auxtr) ->
-    (∀ ρ, fair_model_trace ρ mtr).
-  Proof.
-    intros Hupto Hfa ρ n Hpmod.
-    unfold pred_at in Hpmod.
-    destruct (after n mtr) as [mtr'|] eqn:Heq; last done.
-    destruct (upto_stutter_after _ _ n Hupto Heq) as (n'&auxtr'&Heq'&Hupto').
-    have Hre: role_enabled_model ρ (trfirst mtr') by destruct mtr'.
-    specialize (Hfa ρ).
-    have Henaux : role_enabled ρ (trfirst auxtr').
-    { have HUs: ls_under (trfirst auxtr') = trfirst mtr'.
-      - punfold Hupto'. by inversion Hupto'.
-      - unfold role_enabled, role_enabled_model in *.
-        rewrite HUs //. }
-    have Hfa' := (fair_aux_after ρ auxtr n' auxtr' Hfa Heq' 0).
-    have Hpredat: pred_at auxtr' 0 (λ δ _, role_enabled ρ δ).
-    { rewrite /pred_at /=. destruct auxtr'; done. }
-    destruct (upto_stutter_fairness_0 ρ auxtr' mtr' Hupto' (Hfa' Hpredat)) as (m&Hres).
-    exists m. rewrite !(pred_at_sum _ n) Heq //.
+    - intros. destruct H; [| done]. eauto.
   Qed.
 
-  Lemma upto_stutter_finiteness auxtr (mtr: mtrace M):
-    upto_stutter_aux auxtr mtr ->
-    terminating_trace mtr ->
-    terminating_trace auxtr.
+  (* TODO: move *)
+  Lemma pred_at_iff {St L : Type} (P Q: St -> option L -> Prop)
+    (IFF: forall s ol, P s ol <-> Q s ol):
+      forall tr i, pred_at tr i P <-> pred_at tr i Q.
+  Proof.
+    intros. rewrite /pred_at.
+    destruct after; intuition; destruct t.
+    all: by apply IFF.
+  Qed.
+    
+  Lemma upto_stutter_fairness (eauxtr: eauxtrace (LM := LM)) (emtr: emtrace (EM := EM)):
+    upto_stutter_eauxtr proj_ext eauxtr emtr ->
+    (∀ ρ, fair_eaux ρ eauxtr) ->
+    (* (∀ ρ, fair_model_trace ρ emtr). *)
+    inner_fair_ext_model_trace emtr. 
+  Proof.
+    intros Hupto Hfa.
+    do 2 red. intros ? [ρ ->].
+    do 2 red. intros n Hpmod.
+    unfold pred_at in Hpmod.
+    destruct (after n emtr) as [emtr'|] eqn:Heq
+    (* ; last done. *)
+    .
+    2: { by rewrite Heq in Hpmod. }
+    rewrite Heq in Hpmod.
+    (* Set Printing Implicit. *)
+    assert (role_enabled_model (inl ρ) (trfirst emtr') (M := (@ext_model_FM _ EM))).
+    { by destruct emtr'. }
+    clear Hpmod. rename H into Hpmod. 
+
+    destruct (upto_stutter_after _ _ n Hupto Heq) as (n'&auxtr'&Heq'&Hupto').
+    have Hre: role_enabled_model ρ (trfirst emtr')
+      (* by destruct emtr'. *)
+    .
+    { red. red in Hpmod. simpl in Hpmod. set_solver. }
+    specialize (Hfa ρ).
+    have Henaux : role_enabled ρ (trfirst auxtr').
+    { have HUs: ls_under (trfirst auxtr') = trfirst emtr'.
+      - punfold Hupto'; [| by apply upto_stutter_mono']. 
+        by inversion Hupto'.
+      - unfold role_enabled, role_enabled_model in *.
+        rewrite HUs //. }
+    have Hfa' := (fair_eaux_after ρ eauxtr n' auxtr' Hfa Heq' 0).
+    have Hpredat: pred_at auxtr' 0 (λ δ _, role_enabled ρ δ).
+    { rewrite /pred_at /=. destruct auxtr'; done. }
+    destruct (upto_stutter_fairness_0 ρ auxtr' emtr' Hupto' (Hfa' Hpredat)) as (m&Hres).
+    exists m. rewrite !(pred_at_sum _ n) Heq //.
+    rewrite -pred_at_or. rewrite -pred_at_or in Hres.
+    eapply pred_at_iff; [| apply Hres].
+    intros. simpl. apply or_iff_compat_r. apply not_iff_compat.
+    rewrite {1}/role_enabled_model. simpl. set_solver. 
+  Qed.
+
+  Lemma upto_stutter_finiteness eauxtr (emtr: emtrace (EM := EM)):
+    upto_stutter_eauxtr proj_ext eauxtr emtr ->
+    terminating_trace emtr ->
+    terminating_trace eauxtr.
   Proof.
     intros Hupto [n Hfin].
     have [n' ?] := upto_stutter_after_None _ _ n Hupto Hfin.
